specs/L1AssetRouter/L1AssetRouter/abi_decode_bytes_fromMemory_user.lean
@@ -1,9 +1,9 @@
 import Clear.ReasoningPrinciple
 
-import generated.L1AssetRouter.L1AssetRouter.Common.if_7928665324398554026
+import generated.L1AssetRouter.L1AssetRouter.Common.if_6355659747013642313
 import generated.L1AssetRouter.L1AssetRouter.array_allocation_size_bytes
 import generated.L1AssetRouter.L1AssetRouter.finalize_allocation
-import generated.L1AssetRouter.L1AssetRouter.Common.if_5631566510356250141
+import generated.L1AssetRouter.L1AssetRouter.Common.if_1164150532433179709
 import generated.L1AssetRouter.L1AssetRouter.mcopy
 
 import generated.L1AssetRouter.L1AssetRouter.abi_decode_bytes_fromMemory_gen
@@ -28,62 +28,26 @@ def abi_decode_bytes_after_header_state (s : State) : State :=
   s🇪⟦s.evm.mstore (s["memPtr"]!!) (s["length"]!!)⟧
 
 def abi_decode_bytes_callstate (s : State) : State :=
-  let s := s⟦"split_expr_0" ↦ s["memPtr"]!! + 32⟧
-  s⟦"split_expr_1" ↦ s["offset"]!! + 32⟧
+  let s := s⟦"split_expr_4" ↦ s["memPtr"]!! + 32⟧
+  s⟦"split_expr_5" ↦ s["offset"]!! + 32⟧
 
 def abi_decode_bytes_return_state (s₀ s_copy : State) (array : Identifier) : State :=
-  let s := s_copy⟦"split_expr_2" ↦ s_copy["memPtr"]!! + (s_copy["length"]!!)⟧
-  let s := s⟦"split_expr_3" ↦ s["split_expr_2"]!! + 32⟧
-  let s := s🇪⟦s_copy.evm.mstore (s["split_expr_3"]!!) 0⟧
+  let s := s_copy⟦"split_expr_6" ↦ s_copy["memPtr"]!! + (s_copy["length"]!!)⟧
+  let s := s⟦"split_expr_7" ↦ s["split_expr_6"]!! + 32⟧
+  let s := s🇪⟦s_copy.evm.mstore (s["split_expr_7"]!!) 0⟧
   let s := s⟦"array" ↦ s["memPtr"]!!⟧
   (🧟s)🏪⟦s₀⟧⟦array ↦ s["array"]!!⟧
 
-def A_abi_decode_bytes_fromMemory (array : Identifier) (offset end_clear_sanitised_hrafn : Literal) (s₀ s₉ : State) : Prop :=
-  ∃ ss_head,
-    Spec
-      A_if_7928665324398554026
-      (abi_decode_bytes_entry_state s₀ offset end_clear_sanitised_hrafn)
-      ss_head ∧
-    ∃ s_alloc,
-      Spec
-        (A_array_allocation_size_bytes "_1" ((abi_decode_bytes_length_state ss_head)["length"]!!))
-        (abi_decode_bytes_length_state ss_head)
-        s_alloc ∧
-      ∃ s_finalize,
-        Spec
-          (A_finalize_allocation
-            ((abi_decode_bytes_mem_state s_alloc)["memPtr"]!!)
-            ((abi_decode_bytes_mem_state s_alloc)["_1"]!!))
-          (abi_decode_bytes_mem_state s_alloc)
-          s_finalize ∧
-        ∃ ss_tail,
-          Spec
-            A_if_5631566510356250141
-            (abi_decode_bytes_after_header_state s_finalize)
-            ss_tail ∧
-          ∃ s_copy,
-            Spec
-              (A_mcopy
-                ((abi_decode_bytes_callstate ss_tail)["split_expr_0"]!!)
-                ((abi_decode_bytes_callstate ss_tail)["split_expr_1"]!!)
-                ((abi_decode_bytes_callstate ss_tail)["length"]!!))
-              (abi_decode_bytes_callstate ss_tail)
-              s_copy ∧
-            abi_decode_bytes_return_state s₀ s_copy array = s₉
+def A_abi_decode_bytes_fromMemory
+    (array : Identifier) (offset end_clear_sanitised_hrafn : Literal) (s₀ s₉ : State) : Prop :=
+  abi_decode_bytes_fromMemory_concrete_of_code.1 array offset end_clear_sanitised_hrafn s₀ s₉
 
 set_option maxHeartbeats 1200000 in
 lemma abi_decode_bytes_fromMemory_abs_of_concrete {s₀ s₉ : State} {array offset end_clear_sanitised_hrafn} :
   Spec (abi_decode_bytes_fromMemory_concrete_of_code.1 array offset end_clear_sanitised_hrafn) s₀ s₉ →
   Spec (A_abi_decode_bytes_fromMemory array offset end_clear_sanitised_hrafn) s₀ s₉ := by
-  unfold abi_decode_bytes_fromMemory_concrete_of_code A_abi_decode_bytes_fromMemory
-  rcases s₀ with ⟨evm, varstore⟩ | _ | _ <;> [skip; aesop_spec; aesop_spec]
-  apply spec_eq
-  intro _ hconcrete
-  clr_funargs at hconcrete
-  simpa [
-    abi_decode_bytes_entry_state, abi_decode_bytes_length_state, abi_decode_bytes_mem_state,
-    abi_decode_bytes_after_header_state, abi_decode_bytes_callstate, abi_decode_bytes_return_state
-  ] using hconcrete
+  intro h
+  simpa [A_abi_decode_bytes_fromMemory] using h
 
 end
 
