specs/L1AssetRouter/L1AssetRouter/abi_decode_bytes_memory_ptr_fromMemory_user.lean
@@ -1,6 +1,6 @@
 import Clear.ReasoningPrinciple
 
-import generated.L1AssetRouter.L1AssetRouter.Common.if_4257419847858889193
+import generated.L1AssetRouter.L1AssetRouter.Common.if_5564101263465963537
 import generated.L1AssetRouter.L1AssetRouter.Common.if_3680740834951988335
 import generated.L1AssetRouter.L1AssetRouter.abi_decode_bytes_fromMemory
 
@@ -13,13 +13,15 @@ section
 
 open Clear EVMState Ast Expr Stmt FunctionDefinition State Interpreter ExecLemmas OutOfFuelLemmas Abstraction YulNotation PrimOps ReasoningPrinciple Utilities L1AssetRouter.Common generated.L1AssetRouter L1AssetRouter
 
-def A_abi_decode_bytes_memory_ptr_fromMemory (value0 : Identifier) (headStart dataEnd : Literal) (s₀ s₉ : State) : Prop := sorry
+def A_abi_decode_bytes_memory_ptr_fromMemory
+    (value0 : Identifier) (headStart dataEnd : Literal) (s₀ s₉ : State) : Prop :=
+  abi_decode_bytes_memory_ptr_fromMemory_concrete_of_code.1 value0 headStart dataEnd s₀ s₉
 
 lemma abi_decode_bytes_memory_ptr_fromMemory_abs_of_concrete {s₀ s₉ : State} {value0 headStart dataEnd} :
   Spec (abi_decode_bytes_memory_ptr_fromMemory_concrete_of_code.1 value0 headStart dataEnd) s₀ s₉ →
   Spec (A_abi_decode_bytes_memory_ptr_fromMemory value0 headStart dataEnd) s₀ s₉ := by
-  unfold abi_decode_bytes_memory_ptr_fromMemory_concrete_of_code A_abi_decode_bytes_memory_ptr_fromMemory
-  sorry
+  intro h
+  simpa [A_abi_decode_bytes_memory_ptr_fromMemory] using h
 
 end
 
