specs/L1AssetRouter/L1AssetRouter/fun_bridgehubDepositNonBaseTokenAsset_user.lean
@@ -48,7 +48,8 @@ def A_fun_bridgehubDepositNonBaseTokenAsset
 lemma fun_bridgehubDepositNonBaseTokenAsset_abs_of_concrete {s₀ s₉ : State} {var_request_mpos var_chainId var_originalCaller var_value var__data_offset var_data_1714_length var_nativeTokenVault} :
   Spec (fun_bridgehubDepositNonBaseTokenAsset_concrete_of_code.1 var_request_mpos var_chainId var_originalCaller var_value var__data_offset var_data_1714_length var_nativeTokenVault) s₀ s₉ →
   Spec (A_fun_bridgehubDepositNonBaseTokenAsset var_request_mpos var_chainId var_originalCaller var_value var__data_offset var_data_1714_length var_nativeTokenVault) s₀ s₉ := by
-  simpa [A_fun_bridgehubDepositNonBaseTokenAsset]
+  intro h
+  simpa [A_fun_bridgehubDepositNonBaseTokenAsset] using h
 
 theorem bridgehubDepositNonBaseTokenAsset_preserves_bridged_amount
     {amount : Literal}
